src/lib/crypto/DY.Lib.Crypto.AEAD.Split.fst
@@ -5,6 +5,7 @@ open DY.Core
 open DY.Lib.Crypto.SplitPredicate
 
 let split_aead_predicate_params {|crypto_usages|}: split_crypto_predicate_parameters = {
+  key_t = bytes;
   key_usage_t = key_usage:usage{AeadKey? key_usage};
   data_t = (bytes & bytes & bytes);
   get_usage = (fun key_usage ->
@@ -12,17 +13,23 @@ let split_aead_predicate_params {|crypto_usages|}: split_crypto_predicate_parame
     tag
   );
 
-  local_pred_t = aead_crypto_predicate;
-  global_pred_t = trace -> key_usage:usage{AeadKey? key_usage} -> nonce:bytes -> msg:bytes -> ad:bytes -> prop;
+  key_well_formed = bytes_well_formed;
+  has_usage_split = has_usage;
+  has_usage_split_later = (fun tr1 tr2 key key_usage ->
+    has_usage_later tr1 tr2 key key_usage
+  );
 
-  apply_local_pred = (fun pred (tr, key_usage, (nonce, msg, ad)) ->
-    pred.pred tr key_usage nonce msg ad
+  local_pred_t = aead_crypto_predicate;
+  global_pred_t = tr:trace -> key_usage:usage{AeadKey? key_usage} -> key:bytes{key `has_usage tr` key_usage} -> nonce:bytes -> msg:bytes -> ad:bytes -> prop;
+
+  apply_local_pred = (fun pred (|tr, key_usage, key, (nonce, msg, ad)|) ->
+    pred.pred tr key_usage key nonce msg ad
   );
-  apply_global_pred = (fun pred (tr, key_usage, (nonce, msg, ad)) ->
-    pred tr key_usage nonce msg ad
+  apply_global_pred = (fun pred (|tr, key_usage, key, (nonce, msg, ad)|) ->
+    pred tr key_usage key nonce msg ad
   );
-  mk_global_pred = (fun pred tr key_usage nonce msg ad ->
-    pred (tr, key_usage, (nonce, msg, ad))
+  mk_global_pred = (fun pred tr key_usage key nonce msg ad ->
+    pred (|tr, key_usage, key, (nonce, msg, ad)|)
   );
 
   data_well_formed = (fun tr (nonce, msg, ad) ->
@@ -32,18 +39,18 @@ let split_aead_predicate_params {|crypto_usages|}: split_crypto_predicate_parame
   );
 
   apply_mk_global_pred = (fun bare x -> ());
-  apply_local_pred_later = (fun lpred tr1 tr2 key_usage (nonce, msg, ad) ->
-    lpred.pred_later tr1 tr2 key_usage nonce msg ad
+  apply_local_pred_later = (fun lpred tr1 tr2 key_usage key (nonce, msg, ad) ->
+    lpred.pred_later tr1 tr2 key_usage key nonce msg ad
   );
 }
 
 val has_aead_predicate: {|crypto_invariants|} -> (string & aead_crypto_predicate) -> prop
 let has_aead_predicate #cinvs (tag, local_pred) =
-  forall (tr:trace) (key_usage:usage) (nonce:bytes) (msg:bytes) (ad:bytes).
-    {:pattern aead_pred.pred tr key_usage nonce msg ad}
+  forall (tr:trace) (key_usage:usage) (key:bytes{key `has_usage tr` key_usage}) (nonce:bytes) (msg:bytes) (ad:bytes).
+    {:pattern aead_pred.pred tr key_usage key nonce msg ad}
     match key_usage with
     | AeadKey aead_tag _ ->
-        aead_tag = tag ==> aead_pred.pred tr key_usage nonce msg ad == local_pred.pred tr key_usage nonce msg ad
+        aead_tag = tag ==> aead_pred.pred tr key_usage key nonce msg ad == local_pred.pred tr key_usage key nonce msg ad
     | _ -> True
 
 val intro_has_aead_predicate:
@@ -53,15 +60,15 @@ val intro_has_aead_predicate:
   (ensures has_aead_predicate tagged_local_pred)
 let intro_has_aead_predicate #cinvs (tag, local_pred) =
   introduce
-    forall tr key_usage nonce msg ad.
+    forall tr (key_usage:usage{AeadKey? key_usage}) (key:bytes{key `has_usage tr` key_usage}) nonce msg ad.
       match key_usage with
       | AeadKey aead_tag _ ->
-          aead_tag = tag ==> aead_pred.pred tr key_usage nonce msg ad == local_pred.pred tr key_usage nonce msg ad
+          aead_tag = tag ==> aead_pred.pred tr key_usage key nonce msg ad == local_pred.pred tr key_usage key nonce msg ad
       | _ -> True
   with (
     match key_usage with
     | AeadKey aead_tag _ ->
-      has_local_crypto_predicate_elim split_aead_predicate_params aead_pred.pred tag local_pred tr key_usage (nonce, msg, ad)
+      has_local_crypto_predicate_elim split_aead_predicate_params aead_pred.pred tag local_pred tr key_usage key (nonce, msg, ad)
     | _ -> ()
   )
 
@@ -73,7 +80,7 @@ val mk_aead_predicate:
   aead_crypto_predicate
 let mk_aead_predicate #cusgs l = {
   pred = mk_global_crypto_predicate split_aead_predicate_params l;
-  pred_later = (fun tr1 tr2 key_usg nonce msg ad -> mk_global_crypto_predicate_later split_aead_predicate_params l tr1 tr2 key_usg (nonce, msg, ad));
+  pred_later = (fun tr1 tr2 key_usg key nonce msg ad -> mk_global_crypto_predicate_later split_aead_predicate_params l tr1 tr2 key_usg key (nonce, msg, ad));
 }
 
 val mk_aead_predicate_correct:
