src/lib/crypto/DY.Lib.Crypto.Signature.Split.fst
@@ -5,6 +5,7 @@ open DY.Core
 open DY.Lib.Crypto.SplitPredicate
 
 let split_sign_predicate_params {|crypto_usages|}: split_crypto_predicate_parameters = {
+  key_t = bytes;
   key_usage_t = sk_usage:usage{SigKey? sk_usage};
   data_t = bytes;
   get_usage = (fun vk_usg ->
@@ -12,17 +13,28 @@ let split_sign_predicate_params {|crypto_usages|}: split_crypto_predicate_parame
     tag
   );
 
-  local_pred_t = sign_crypto_predicate;
-  global_pred_t = tr:trace -> sk_usage:usage{SigKey? sk_usage} -> msg:bytes -> prop;
+  key_well_formed = bytes_well_formed;
+  has_usage_split = has_signkey_usage;
+  has_usage_split_later = (fun tr1 tr2 vk sk_usage ->
+    normalize_term_spec bytes_well_formed;
+    match vk with
+    | Vk sk -> (
+      get_usage_later tr1 tr2 sk
+    )
+    | _ -> ()
+  );
 
-  apply_local_pred = (fun pred (tr, sk_usage, msg) ->
-    pred.pred tr sk_usage msg
+  local_pred_t = sign_crypto_predicate;
+  global_pred_t = tr:trace -> sk_usage:usage{SigKey? sk_usage} -> vk:bytes{vk `has_signkey_usage tr` sk_usage} -> msg:bytes -> prop;
+
+  apply_local_pred = (fun pred (|tr, sk_usage, sk, msg|) ->
+    pred.pred tr sk_usage sk msg
   );
-  apply_global_pred = (fun pred (tr, sk_usage, msg) ->
-    pred tr sk_usage msg
+  apply_global_pred = (fun pred (|tr, sk_usage, sk, msg|) ->
+    pred tr sk_usage sk msg
   );
-  mk_global_pred = (fun pred tr sk_usage msg ->
-    pred (tr, sk_usage, msg)
+  mk_global_pred = (fun pred tr sk_usage sk msg ->
+    pred (|tr, sk_usage, sk, msg|)
   );
 
   data_well_formed = (fun tr msg ->
@@ -37,11 +49,11 @@ let split_sign_predicate_params {|crypto_usages|}: split_crypto_predicate_parame
 
 val has_sign_predicate: {|crypto_invariants|} -> (string & sign_crypto_predicate) -> prop
 let has_sign_predicate #cinvs (tag, local_pred) =
-  forall (tr:trace) (sk_usage:usage) (msg:bytes).
-    {:pattern sign_pred.pred tr sk_usage msg}
+  forall (tr:trace) (sk_usage:usage) (vk:bytes{vk `has_signkey_usage tr` sk_usage}) (msg:bytes).
+    {:pattern sign_pred.pred tr sk_usage vk msg}
     match sk_usage with
     | SigKey sign_tag _ ->
-        sign_tag = tag ==> sign_pred.pred tr sk_usage msg == local_pred.pred tr sk_usage msg
+        sign_tag = tag ==> sign_pred.pred tr sk_usage vk msg == local_pred.pred tr sk_usage vk msg
     | _ -> True
 
 val intro_has_sign_predicate:
@@ -51,15 +63,15 @@ val intro_has_sign_predicate:
   (ensures has_sign_predicate tagged_local_pred)
 let intro_has_sign_predicate #cinvs (tag, local_pred) =
   introduce
-    forall tr sk_usage msg.
+    forall tr sk_usage vk msg.
       match sk_usage with
       | SigKey sign_tag _ ->
-          sign_tag = tag ==> sign_pred.pred tr sk_usage msg == local_pred.pred tr sk_usage msg
+          sign_tag = tag ==> sign_pred.pred tr sk_usage vk msg == local_pred.pred tr sk_usage vk msg
       | _ -> True
   with (
     match sk_usage with
     | SigKey sign_tag _ ->
-      has_local_crypto_predicate_elim (split_sign_predicate_params) sign_pred.pred tag local_pred tr sk_usage msg
+      has_local_crypto_predicate_elim (split_sign_predicate_params) sign_pred.pred tag local_pred tr sk_usage vk msg
     | _ -> ()
   )
 
@@ -71,7 +83,9 @@ val mk_sign_predicate:
   sign_crypto_predicate
 let mk_sign_predicate #cusgs l = {
   pred = mk_global_crypto_predicate split_sign_predicate_params l;
-  pred_later = mk_global_crypto_predicate_later split_sign_predicate_params l;
+  pred_later = (fun tr1 tr2 sk_usage vk msg ->
+    mk_global_crypto_predicate_later split_sign_predicate_params l tr1 tr2 sk_usage vk msg
+  );
 }
 
 val mk_sign_predicate_correct:
